Phi_System/Phi_Type_Algebra.thy
@@ -890,11 +890,9 @@ lemma [\<phi>reason_template default 50 requires Separation_Homo\<^sub>E]:
 
 lemma [\<phi>reason_template default 45]:
   \<open> Separation_Homo\<^sub>E Fa\<^sub>L Fa\<^sub>R Fb un
-\<Longrightarrow> x \<Ztypecolon> Fb (U\<^sub>L \<^emph>\<^sub>\<A> U\<^sub>R) \<t>\<r>\<a>\<n>\<s>\<f>\<o>\<r>\<m>\<s> y \<Ztypecolon> Fa\<^sub>L U\<^sub>L \<^emph>\<^sub>\<A> Fa\<^sub>R U\<^sub>R \<s>\<u>\<b>\<j> y. (\<exists>z. y = un z) @action \<A>simp\<close>
+\<Longrightarrow> x \<Ztypecolon> Fb (U\<^sub>L \<^emph>\<^sub>\<A> U\<^sub>R) \<t>\<r>\<a>\<n>\<s>\<f>\<o>\<r>\<m>\<s> y \<Ztypecolon> Fa\<^sub>L U\<^sub>L \<^emph>\<^sub>\<A> Fa\<^sub>R U\<^sub>R \<s>\<u>\<b>\<j> y. y = un x @action \<A>simp\<close>
   unfolding Separation_Homo\<^sub>E_def Action_Tag_def \<phi>Auto_Prod_def
-  by (clarsimp simp add: Subjection_transformation_expn Ex_transformation_expn
-                  intro!: ExSet_transformation_I Subjection_imp_I,
-      rule transformation_weaken[where P=True], blast, blast)
+  by (clarsimp simp add: Subjection_transformation_expn Ex_transformation_expn)
 
 
 locale Functional_Transformation_Functor =
@@ -1600,7 +1598,8 @@ lemma \<phi>TA_TF_pattern_IH:
 
 lemma \<phi>TA_TF_rule_step:
   \<open> X \<t>\<r>\<a>\<n>\<s>\<f>\<o>\<r>\<m>\<s> X' \<w>\<i>\<t>\<h> Any @action \<A>_every_item A
-\<Longrightarrow> X' \<t>\<r>\<a>\<n>\<s>\<f>\<o>\<r>\<m>\<s> Y @action NToA
+\<Longrightarrow> X' \<t>\<r>\<a>\<n>\<s>\<f>\<o>\<r>\<m>\<s> X'' \<w>\<i>\<t>\<h> Any' @action \<A>_apply_simplication
+\<Longrightarrow> X'' \<t>\<r>\<a>\<n>\<s>\<f>\<o>\<r>\<m>\<s> Y @action NToA
 \<Longrightarrow> X \<t>\<r>\<a>\<n>\<s>\<f>\<o>\<r>\<m>\<s> Y @action A\<close>
   unfolding Action_Tag_def
   by (simp add: Transformation_def)
